First attempt at histories and corresponding events

src/semantics.lean
@@ -53,16 +53,15 @@ inductive vallist (β : Type) [objects α β] :
   value β ty → vallist l → vallist (ty::l)
 structure object_space (β : Type) [objects α β]
     (self : class_name α) :=
-  (this : value β (ref self))
+  (val : value β (ref self))
   (state : state_space β self)
 
-variables {self : class_name α} {o : object_space β self}
-variable {e : tenv self}
+variables {self : class_name α}
 
 /- An active process consists of: an argument space (of the current method), a value list (of the local variables), and a statement. -/
-structure active_process (o : object_space β self) (e : tenv self) :=
-  (args : arg_space β e.current)
-  (store : vallist β e.locals)
+structure active_process (this : object_space β self)
+    (e : tenv self) :=
+  (args : arg_space β e.current) (store : vallist β e.locals)
   (stmt : stmt e)
 /- Given a value list and an index in the list of types, we obtain a value. -/
 def vallist.lookup : Π {l : context α} {ty : type α},
@@ -73,33 +72,35 @@ def vallist.lookup : Π {l : context α} {ty : type α},
   (list_at.tail .(x) (zs : list_at .(ty) xs)) :=
     vallist.lookup ys zs
 -- Given an active process, we can lookup the value of a read variable.
-def active_process.lookup  (P : active_process o e)
+variables {this : object_space β self} {e : tenv self}
+def active_process.lookup (P : active_process this e)
     {tx : type α} : rvar e tx → value β tx
-| (rvar.tvar t) := eq.mpr (congr_arg _ t.H) o.this
-| (rvar.fvar f) := eq.mpr (congr_arg _ f.H) $ o.state.map f.idx
+| (rvar.tvar t) := eq.mpr (congr_arg _ t.H) this.val
+| (rvar.fvar f) := eq.mpr (congr_arg _ f.H) $ this.state.map f.idx
 | (rvar.pvar p) := eq.mpr (congr_arg _ p.H) $ P.args.map p.idx
 | (rvar.lvar l) := P.store.lookup l.idx
 /- Evaluating a pure expression in an active process. -/
-def eval (P : active_process o e) : Π {ty : type α},
+def eval (P : active_process this e) : Π {ty : type α},
     pexp e ty → value β ty
 | bool (requal l r) := value.term β $ to_bool (eval l = eval r)
 | _ (lookup r) := P.lookup r
 | _ (const _ v) := value.term β v
 | _ (apply f r) := value.term β $ f (eval r).unterm
 /- A process is either nil or an active process. -/
-inductive process (o : object_space β self)
+inductive process (this : object_space β self)
 | nil : process
-| active {e : tenv self} (a : active_process o e) : process
+| active {e : tenv self} (a : active_process this e) : process
 /- A local configuration is an object configuration and a process. -/
 structure local_config (α β : Type) [objects α β] :=
-  (self : class_name α) (o : object_space β self)
-  (m : process o)
+  (self : class_name α)(this : object_space β self)
+  (m : process this)
 /- A global history is a sequence of events. An event is either an asynchronous method call of some caller object to a callee object, its method, and for each parameter an argument value. Or, an event is a method selection. -/
 @[derive decidable_eq]
 structure callsite (α β : Type) [objects α β] :=
   (o : β)
   (m : method_name (class_of α o))
   (τ : arg_space β m)
+@[derive decidable_eq]
 inductive event (α β : Type) [objects α β]
 | call: β → callsite α β → event
 | selection: callsite α β → event
@@ -108,37 +109,77 @@ def event.to_callsite : event α β → callsite α β
 | (event.selection c) := c
 instance event.event_to_callsite : has_coe (event α β)
   (callsite α β) := ⟨event.to_callsite⟩
-open event
 /- Given an object, we consider two subsequences of a global history. The first consists only of call events with the object as callee (abstracted to its corresponding call site), the second consists only of selection events with the object as callee. -/
+@[simp]
 def event.is_call_to (α : Type) [objects α β] (x : β) :
     event α β → option (callsite α β)
-| (call o c) := if x = c.o then c else none
+| (event.call _ c) := if x = c.o then some c else none
 | _ := none
+@[simp]
 def event.is_selection_of (α : Type) [objects α β] (x : β) :
     event α β → option (callsite α β)
-| (selection c) := if x = c.o then c else none
+| (event.selection c) := if x = c.o then some c else none
 | _ := none
+@[simp]
 def event.calls_to (x : list (event α β)) (o : β) :
     list (callsite α β) :=
   x.filter_map (event.is_call_to α o)
-notation x `?`:100 o := event.calls_to x o
+notation x `!`:68 o:69 := event.calls_to x o
+@[simp]
 def event.selections_of (x : list (event α β))
     (o : β) : list (callsite α β) :=
   x.filter_map (event.is_selection_of α o)
-notation x `!`:100 o := event.selections_of x o
+notation x `?`:68 o:69 := event.selections_of x o
 /- A global history is a sequence of events, restricted to those in which for each object, the subsequence of calls to is a prefix of the subsequence of selections. -/
-structure global_history (α β : Type) [objects α β] :=
-(seq : list (event α β))
-(wellformed : ∀ o : β, is_prefix (seq?o) (seq!o))
+@[reducible]
+def global_history (α β : Type) [objects α β] :=
+  {seq : list (event α β) // ∀ o : β, is_prefix (seq?o) (seq!o)}
 /- Given a global history and an object, a call site is pending if the number of occurrences in calls is higher than the number of occurrences in selections. -/
-def global_history.is_pending (x : global_history α β)
+def global_history.is_pending (θ : global_history α β)
     (c : callsite α β) : Prop :=
-  length (filter (= c) (x.seq?c.o)) >
-  length (filter (= c) (x.seq!c.o))
+  length (filter (= c) (θ?c.o)) >
+  length (filter (= c) (θ!c.o))
+/- Given a non-empty global history, a selection event is never first. -/
+lemma global_history.never_selection (seq : list (event α β))
+  (c : callsite α β) : ¬∀ o : β, is_prefix
+  ((event.selection c::seq)?o) ((event.selection c::seq)!o) :=
+begin
+  admit -- TODO
+end
+/- Given a global history and an object identity, a scheduler scheduler takes the first pending call, if any. To do so we match each call event with the first corresponding selection event, cancelling them if they both occur. If no corresponding selection event is found, we have found a pending call. -/
+def global_history.cancel: callsite α β → list (event α β) →
+    option (list (event α β))
+| _ [] := none
+| c (d :: l) := if c = d then (some l)
+    else option.map (cons d) (global_history.cancel c l)
+-- TODO: proof that global_history.cancel can be lifted to global histories
+def global_history.sched : global_history α β → β →
+    option (callsite α β)
+| ⟨[], _⟩ _ := none
+| ⟨(event.selection c) :: l, H⟩ o' :=
+  begin
+    exfalso, apply global_history.never_selection l c, apply H
+  end
+| ⟨e@(event.call o _) :: l, _⟩ o' :=
+  match global_history.cancel ↑e l with
+  | none := e
+  | (some l') := sorry -- global_history.sched l'
+  end
+/- A local step is taken on a local configuration and a corresponding local history, to a next local configuration. -/
+def local_step (x : local_config α β) : local_config α β :=
+  sorry
 /- A global configuration is a finite set of object configurations and a global history. -/
 structure global_config (α β : Type) [objects α β] :=
   (Γ: finset (local_config α β))
   (θ: global_history α β)
-/- A local step is a map from local configuration to local configuration. -/
-def local_step (x : local_config α β) : local_config α β :=
-  sorry
+/- A local history is obtained from a global history and an object identity: it consists of the outgoing calls, an method selections involving the object. -/
+@[reducible]
+def event.is_local_to (α : Type) [objects α β] (x : β) :
+    event α β → Prop
+| (event.call y _) := x = y -- same caller
+| (event.selection c) := x = c.o -- same callee
+instance event.decidable_local (o : β) (e: event α β) :
+    decidable (event.is_local_to α o e) :=
+  begin cases e; apply_instance end
+def local_history (θ : global_history α β) (o : β) :=
+  filter (event.is_local_to α o) θ
